SPos/Syntax/Syntax.lean
@@ -4,6 +4,10 @@ inductive Tm : (n : Nat) → Type where
 | pi  : Tm n → Tm (n + 1) → Tm n
 | lam : Tm n → Tm (n + 1) → Tm n
 | app : Tm n → Tm n → Tm n
+-- Identity
+| id   : Tm n → Tm n → Tm n → Tm n
+| refl : Tm n → Tm n → Tm n
+| j    : Tm (n + 2) → Tm n → Tm n → Tm n
 -- Universe
 | u  : Nat → Tm n
 
@@ -15,6 +19,10 @@ infixr:(max - 1) "•" => Tm.app
 
 prefix:(max - 1) "𝓤" => Tm.u
 
+notation "Id" => Tm.id
+notation "refl" => Tm.refl
+notation "J" => Tm.j
+
 def Ren (n m : Nat) := Fin n → Fin m
 
 def Ren.lift (ρ : Ren n m) : Ren (n + 1) (m + 1) :=
@@ -25,6 +33,9 @@ def Tm.rename (ρ : Ren n m) : Tm n → Tm m
 | .pi τ υ    => .pi (τ.rename ρ) (υ.rename ρ.lift)
 | .lam τ t   => .lam (τ.rename ρ) (t.rename ρ.lift)
 | .app t₁ t₂ => .app (t₁.rename ρ) (t₂.rename ρ)
+| .id τ a b  => .id (τ.rename ρ) (a.rename ρ) (b.rename ρ)
+| .refl τ a  => .refl (τ.rename ρ) (a.rename ρ)
+| .j c d p   => .j (c.rename ρ.lift.lift) (d.rename ρ) (p.rename ρ)
 | .u ℓ       => .u ℓ
 
 def Tm.weaken : Tm n → Tm (n + 1) := Tm.rename Fin.succ
@@ -41,6 +52,9 @@ def Tm.subst (σ : Subst n m) : Tm n → Tm m
 | .pi τ υ    => .pi (τ.subst σ) (υ.subst σ.lift)
 | .lam τ t   => .lam (τ.subst σ) (t.subst σ.lift)
 | .app t₁ t₂ => .app (t₁.subst σ) (t₂.subst σ)
+| .id τ a b  => .id (τ.subst σ) (a.subst σ) (b.subst σ)
+| .refl τ a  => .refl (τ.subst σ) (a.subst σ)
+| .j c d p   => .j (c.subst σ.lift.lift) (d.subst σ) (p.subst σ)
 | .u ℓ       => .u ℓ
 
 def Subst.single (u : Tm n) : Subst (n + 1) n :=
